[minor] More progress in refinement proof.
Still not compiling...

compartmentalization/refinementSA.v
@@ -15,6 +15,8 @@ Import DoNotation.
 Section RefinementSA.
 
 Set Implicit Arguments.
+Unset Strict Implicit.
+Unset Printing Implicit Defensive.
 
 Import PartMaps.
 Import Abs.Notations.
@@ -120,6 +122,7 @@ Proof.
 Qed.
 *)
 
+(*
 Definition the {T : finType} (xs : {set T}) : option T :=
   [pick a | xs == [set a]].
 
@@ -134,24 +137,17 @@ Qed.
 Definition map_options {T S : finType} (f : T -> option S) (xs : {set T}) : option {set S} :=
   if None \in f @: xs then None
   else Some [set a | Some a \in f @: xs].
-
-
-
+*)
 
 Definition refined_compartment (c   : Abs.compartment t)
                                (sst : sstate) : option word :=
   let: <<A,J,S>> := c in
-  [pick sc in [
+  [pick sc |
 
-
-  do! sc  <- the =<< map_options (stag_compartment ∘ slabel <=< Sym.sget sst) A;
-             (* modulo emptiness *)
-  do! guard? all (fun s : {set word} => sc \in s) <$>
-             map_options (stag_incoming ∘ slabel <=< Sym.sget sst) J;
-  do! guard? all (fun s : {set word} => sc \in s) <$>
-             map_options (stag_writers  ∘ slabel <=< Sym.sget sst) S;
-  Some sc.
-End With_EqType_refined_compartment.
+    [set Some sc] == (stag_compartment ∘ slabel <=< Sym.sget sst) @: A &
+    [forall os in (stag_incoming ∘ slabel <=< Sym.sget sst) @: J :|:
+                  (stag_writers  ∘ slabel <=< Sym.sget sst) @: S,
+     oapp (fun s : {set word} => sc \in s) false os] ].
 
 Definition refine_compartment_tag (C   : list (Abs.compartment t))
                                   (sst : sstate)
@@ -176,6 +172,8 @@ Definition refine_compartment_tag (C   : list (Abs.compartment t))
     | None =>
       True
   end.
+
+End With_EqType_refined_compartment.
 
 Definition refine_compartments (C : list (Abs.compartment t))
                                (sst : sstate) : Prop :=
@@ -219,6 +217,7 @@ Record refine (ast : astate) (sst : sstate) : Prop := RefineState
 
 Generalizable All Variables.
 
+(*
 (* MOVE *)
 Lemma map_options_in (X Y : eqType) (f : X -> option Y) xs ys :
   map_options f xs = Some ys ->
@@ -243,6 +242,7 @@ Proof.
         case/orP: H2 => [/eqP E | //].
         congruence.
 Qed.
+*)
 
 Ltac explode_refined_compartment' RC :=
   let sxs      := fresh "sxs"      in
@@ -295,11 +295,11 @@ Lemma refined_sget_in_compartment : forall C c cid sst x I W p,
   C ⊢ p ∈ c.
 Proof.
   clear S I.
-  move=> C c cid sst x I W p GOODS IN_c_C RCTAGS REFINED SGET.
+  move=> C [A J S] cid sst x I W p GOODS IN_c_C RCTAGS /= REFINED SGET.
   move: (RCTAGS p) => RCTAGS'; rewrite /refine_compartment_tag SGET in RCTAGS';
     move: RCTAGS' => [c' [IC' RTAG]].
-  let S := fresh "S" in explode_refined_compartment REFINED A J S.
-  move/(the_in _)/MAP_sxs: def_sc => [[w Lw] TAG /def_sxs [p' SGET' IN']].
+  case: pickP REFINED => //= cid' /andP [? /forallP ?].
+  admit. (*
   have IC_p'_c : C ⊢ p' ∈ <<A,J,S>>.  rewrite /Abs.in_compartment /=.
   move: (mem_enum A).
 
@@ -313,14 +313,14 @@ IN'. by apply Abs.in_compartment_spec.
   inversion TAG; subst.
   move: RTAG => [SAME _]; assert (IC_p'_c' : C ⊢ p' ∈ c') by by apply SAME.
   replace c' with <<A,J,S>> in * by eauto 3.
-  assumption.
+  assumption.*)
 Qed.
 
 Theorem refine_good : forall `(REFINE : refine ast sst),
   Abs.good_state ast ->
   Sym.good_state sst.
 Proof.
-  clear S I.
+  clear S I. admit. (*
   move=> [Apc AR AM AC Ask Aprev]
          [SM SR [Spc Lpc] [Snext SiT SaJT SaST]]
          [RPC RREGS RMEMS RCOMPS RPREV RSC RINT]
@@ -386,7 +386,7 @@ Proof.
         inversion GET; subst;
         simpl in TAG; inversion TAG; subst;
         eauto.
-  - assumption.
+  - assumption.*)
 Qed.
 
 Ltac unoption :=
@@ -404,19 +404,18 @@ Lemma prove_refined_compartment : forall pc instr cid I W
   forallb (is_some ∘ refined_compartment^~ sst) AC ->
   (forall p, refine_compartment_tag AC sst p) ->
   AC ⊢ pc ∈ c ->
-  is_set I ->
   (forall p' : word,
      match Sym.sget sst p' with
        | Some _@(Sym.PC _ _) => False
        | Some _@(Sym.DATA cid' I' W') =>
          (cid = cid' <-> AC ⊢ p' ∈ c) /\
-         (In cid I' -> In p' (Abs.jump_targets c)) /\
-         (In cid W' -> In p' (Abs.store_targets c))
+         (cid \in I' -> p' \in Abs.jump_targets c) /\
+         (cid \in W' -> p' \in Abs.store_targets c)
        | Some _@Sym.REG => False
        | None => True
      end) ->
   refined_compartment c sst ?= cid.
-Proof.
+Proof. admit. Qed. (*
   clear S I; intros until 0; simpl in *;
     intros PC AGOOD RCOMPS RCTAGS IN_c SET_I RTAG;
     rewrite /refine_compartment_tag in RCTAGS; simpl in *.
@@ -446,33 +445,33 @@ Proof.
     destruct RTAG as [SAME _].
     symmetry; apply SAME; assumption.
 Qed.
+*)
 
 Lemma prove_refined_compartment' : forall pc instr cid cid' cid'' I W F
                                           AR AM AC Ask Aprev c sst,
   Sym.sget sst pc ?= instr@(Sym.DATA cid'' I W) ->
-  (do! guard (cid'' == cid') || ((F == JUMPED) && set_elem cid' I);
+  (do! guard (cid'' == cid') || ((F == JUMPED) && (cid' \in I));
    Some cid'') ?= cid ->
   Abs.good_state (AState pc AR AM AC Ask Aprev) ->
   forallb (is_some ∘ refined_compartment^~ sst) AC ->
   (forall p, refine_compartment_tag AC sst p) ->
   AC ⊢ pc ∈ c ->
-  is_set I ->
   (forall p' : word,
      match Sym.sget sst p' with
        | Some _@(Sym.PC _ _) => False
        | Some _@(Sym.DATA cid''' I' W') =>
          (cid'' = cid''' <-> AC ⊢ p' ∈ c) /\
-         (In cid'' I' -> In p' (Abs.jump_targets c)) /\
-         (In cid'' W' -> In p' (Abs.store_targets c))
+         (cid'' \in I' -> p' \in Abs.jump_targets c) /\
+         (cid'' \in W' -> p' \in Abs.store_targets c)
        | Some _@Sym.REG => False
        | None => True
      end) ->
   refined_compartment c sst == Some cid.
-Proof.
+Proof. admit. Qed. (*
   intros until 0; intros SGET GUARD.
   undo1 GUARD COND; inversion GUARD; subst.
   intros; apply/eqP; eapply prove_refined_compartment; eauto.
-Qed.
+Qed.*)
 
 Lemma prove_permitted_now_in : forall pc instr cid cid' cid'' I W F
                                       AR AM AC Ask Aprev
@@ -481,25 +480,24 @@ Lemma prove_permitted_now_in : forall pc instr cid cid' cid'' I W F
   let sst := (SState mem reg pc@(Sym.PC F cid') int) in
   Sym.sget sst pc ?= instr@(Sym.DATA cid'' I W) ->
   (Ask == F) && (refined_compartment Aprev sst == Some cid') ->
-  (do! guard (cid'' == cid') || ((F == JUMPED) && set_elem cid' I);
+  (do! guard (cid'' == cid') || ((F == JUMPED) && (cid' \in I));
    Some cid'') ?= cid ->
   Abs.good_state (AState pc AR AM AC Ask Aprev) ->
   Sym.good_state sst ->
   (forall p, refine_compartment_tag AC sst p) ->
   AC ⊢ pc ∈ c ->
-  is_set I ->
   (forall p' : word,
      match Sym.sget sst p' with
       | Some _@(Sym.PC _ _) => False
       | Some _@(Sym.DATA cid''' I' W') =>
           (cid'' = cid''' <-> AC ⊢ p' ∈ c) /\
-          (In cid'' I' -> In p' (Abs.jump_targets c)) /\
-          (In cid'' W' -> In p' (Abs.store_targets c))
+          (cid'' \in I' -> p' \in Abs.jump_targets c) /\
+          (cid'' \in W' -> p' \in Abs.store_targets c)
       | Some _@Sym.REG => False
       | None => True
      end) ->
   Abs.permitted_now_in AC Ask Aprev pc ?= c.
-Proof.
+Proof. admit. Qed. (*
   clear S I; intros until 0; subst sst;
     intros PC RPREV def_cid AGOOD SGOOD RCTAGS IN_c SET_I RTAG;
     rewrite /refine_compartment_tag in RCTAGS; simpl in *.
@@ -562,6 +560,7 @@ Proof.
     apply IN_I in IN.
     by assert (c' = <<Aprev,Jprev,Sprev>>) by eauto 3; subst.
 Qed.
+*)
 
 Lemma refined_reg_value : forall AR SR,
   refine_registers AR SR ->
@@ -626,22 +625,18 @@ Definition tags_subsets (sst1 sst2 : sstate) : Prop :=
   forall p,
     match Sym.sget sst1 p , Sym.sget sst2 p with
       | Some _@(Sym.DATA c1 I1 W1) , Some _@(Sym.DATA c2 I2 W2) =>
-        c1 = c2 /\
-        (forall a, In a I1 -> In a I2) /\
-        (forall a, In a W1 -> In a W2)
+        c1 = c2 /\ I1 \subset I2 /\ W1 \subset W2
       | None , None =>
         True
       | _ , _ =>
         False
     end.
 
-Definition tags_subsets_in (ps : list word) (sst1 sst2 : sstate) : Prop :=
+Definition tags_subsets_in (ps : {set word}) (sst1 sst2 : sstate) : Prop :=
   forall p,
     match Sym.sget sst1 p , Sym.sget sst2 p with
       | Some _@(Sym.DATA c1 I1 W1) , Some _@(Sym.DATA c2 I2 W2) =>
-        (In p ps -> c1 = c2) /\
-        (forall a, In a I1 -> In a I2) /\
-        (forall a, In a W1 -> In a W2)
+        (p \in ps -> c1 = c2) /\ I1 \subset I2 /\ W1 \subset W2
       | None , None =>
         True
       | _ , _ =>
@@ -653,8 +648,7 @@ Definition tags_subsets_cid (cid : word) (sst1 sst2 : sstate) : Prop :=
     match Sym.sget sst1 p , Sym.sget sst2 p with
       | Some _@(Sym.DATA c1 I1 W1) , Some _@(Sym.DATA c2 I2 W2) =>
         (c1 = cid \/ c2 = cid -> c1 = c2) /\
-        (forall a, In a I1 -> In a I2) /\
-        (forall a, In a W1 -> In a W2)
+        I1 \subset I2 /\ W1 \subset W2
       | None , None =>
         True
       | _ , _ =>
@@ -662,7 +656,7 @@ Definition tags_subsets_cid (cid : word) (sst1 sst2 : sstate) : Prop :=
     end.
 
 Lemma tags_subsets_in_tail : forall p ps sst sst',
-  tags_subsets_in (p :: ps) sst sst' ->
+  tags_subsets_in (p |: ps) sst sst' ->
   tags_subsets_in ps sst sst'.
 Proof.
   rewrite /tags_subsets_in /=; move=> p ps sst sst' TSI a.
@@ -670,7 +664,9 @@ Proof.
   destruct (Sym.sget sst  a) as [[x  []]|],
            (Sym.sget sst' a) as [[x' []]|];
     try done.
-  move: TSI => [EQ [? ?]]; repeat split; auto.
+  move: TSI => [EQ [? ?]]; repeat split; auto => Hin.
+  suff: a \in p |: ps by auto.
+  by rewrite in_setU1 Hin orbT.
 Qed.
 
 Lemma tags_subsets_trans : forall sst sst' sst'',
@@ -685,6 +681,7 @@ Proof.
            (Sym.sget sst'' p) as [[? []]|];
     try done.
   repeat invh and; subst; auto.
+  admit.
 Qed.
 
 Lemma tags_subsets_in_trans : forall ps sst sst' sst'',
@@ -697,11 +694,11 @@ Proof.
   destruct (Sym.sget sst   p) as [[? []]|],
            (Sym.sget sst'  p) as [[? []]|],
            (Sym.sget sst'' p) as [[? []]|];
-    try done.
+    try done. admit. (*
   destruct (elem p ps); repeat invh and;
   repeat match goal with IN : In p ps, H : In p ps -> _ |- _ =>
     specialize (H IN)
-  end; subst; repeat split; auto; done.
+  end; subst; repeat split; auto; done.*)
 Qed.
 
 Lemma tags_subsets_any_in : forall ps sst sst',
@@ -724,7 +721,7 @@ Lemma refined_compartment_untouched_preserved : forall sst sst' c cid,
 Proof.
   clear S I; intros sst sst' [A J S] cid GOOD GOOD' TSI.
   rewrite /refined_compartment /=.
-
+  admit. (*
   assert (INIT :
     (do! sxs <- map_options (Sym.sget sst) A;
      the =<< map_options (Sym.stag_compartment ∘ slabel) sxs)
@@ -814,7 +811,7 @@ Proof.
   lapply EQ_ALL_J; [clear EQ_ALL_J; intro ALL_J' | done].
   lapply EQ_ALL_S; [clear EQ_ALL_S; intro ALL_S' | done].
   destruct (forallb _ <$> MAP_J') as [[]|]; try done.
-  destruct (forallb _ <$> MAP_S') as [[]|]; done.
+  destruct (forallb _ <$> MAP_S') as [[]|]; done. *)
 Qed.
 
 Lemma refined_compartment_all_untouched_preserved : forall sst sst' c cid,
@@ -849,6 +846,7 @@ Proof.
   clear S I; intros sst sst' [A J S] SAME.
   rewrite /equilabeled in SAME.
   rewrite /refined_compartment /=.
+  admit. (*
   assert (INIT :
     (do! sxs <- map_options (Sym.sget sst) A;
      the =<< map_options (Sym.stag_compartment ∘ slabel) sxs)
@@ -883,7 +881,7 @@ Proof.
     simpl in SAME; inversion SAME; subst; simpl.
     by rewrite IHS'.
   }
-  rewrite bind_assoc INIT -bind_assoc EQ_MAP_J EQ_MAP_S; reflexivity.
+  rewrite bind_assoc INIT -bind_assoc EQ_MAP_J EQ_MAP_S; reflexivity.*)
 Qed.
 
 Lemma refined_compartment_irrelevancies : forall c SM SR SR' Spc Spc'
@@ -909,6 +907,7 @@ Proof.
   destruct (Sym.sget sst  p) as [[x  [|cid  I  W|]]|],
            (Sym.sget sst' p) as [[x' [|cid' I' W'|]]|];
     try done.
+  admit. (*
   move: GMEM_p GMEM'_p => _ /andP [SET_I' SET_W'].
   repeat split; auto.
   destruct RCT as [SET_I [SET_W [c [IC RTAG]]]].
@@ -917,9 +916,10 @@ Proof.
   move=> q; move: (TS q) (RTAG q) => TS_q RTAG_q.
   destruct (Sym.sget sst  q) as [[y  [|did  K  V|]]|],
            (Sym.sget sst' q) as [[y' [|did' K' V'|]]|];
-    try done.
+    try done. *)
 Abort.
 
+(*
 Lemma forallb_map_options_insert_unique : forall {A B} `{ord : Ordered A}
                                                  p (f : A -> option B) xs a,
   (p <$> f a) ?= true ->
@@ -972,6 +972,7 @@ Proof.
       by rewrite fx in IN'.
     + reflexivity.
 Qed.
+*)
 
 Theorem isolate_create_set_refined : forall AM SM,
   refine_memory AM SM ->
@@ -1033,22 +1034,25 @@ Qed.
 
 Lemma in_compartment_update A J Sa J' Sa' AC p c :
   AC ⊢ p ∈ c ->
-  exists c', <<A,J,Sa>> :: delete <<A,J',Sa'>> AC ⊢ p ∈ c'.
+  exists c', <<A,J,Sa>> :: rem <<A,J',Sa'>> AC ⊢ p ∈ c'.
 Proof.
-  elim => {c AC} [c A'' J'' Sa'' IN|AC c c' IN [c''' IN']] /=.
-  - destruct (SetoidDec.equiv_dec A A'') as [EQ | NEQ].
-    + simpl in EQ. subst. eexists. by constructor.
-    + simpl in NEQ.
-      exists <<A'',J'',Sa''>>.
-      destruct (SetoidDec.equiv_dec <<A,J',Sa'>> <<A'',J'',Sa''>>);
-        first by congruence.
-      by repeat constructor.
-  - inversion IN'; subst.
-    + eexists. by econstructor.
-    + eexists c'''.
-      constructor.
-      destruct (SetoidDec.equiv_dec <<A,J',Sa'>> c); first by trivial.
-      by constructor.
+  elim: AC => [|c' AC IH]; first by rewrite /Abs.in_compartment andbF.
+  rewrite /Abs.in_compartment in_cons => /andP [Has /orP [/eqP <-| Hin]].
+  - rewrite /=.
+    have [E|NE] := altP (c =P <<A,J',Sa'>>).
+    + exists <<A,J,Sa>> => /=.
+      rewrite E in Has.
+      by rewrite Has /= in_cons eqxx.
+    + exists c.
+      by rewrite Has /= !inE eqxx orbT.
+  - have /IH {IH} [c'' /andP [? Hin']] : AC ⊢ p ∈ c by rewrite /Abs.in_compartment Has Hin.
+    exists c''.
+    apply/andP; split => //.
+    rewrite !inE in Hin' *.
+    case/orP: Hin' => [-> //| Hin' /=].
+    have [E|NE] := altP (c' =P <<A,J',Sa'>>).
+    + by rewrite (mem_rem Hin') orbT.
+    + by rewrite inE Hin' !orbT.
 Qed.
 
 Theorem add_to_jump_targets_refined : forall ast sst sst',
@@ -1065,14 +1069,11 @@ Proof.
            ast    as [Apc AR    AM    AC    Ask Aprev],
            sst    as [SM SR Spc [Snext SiT SaJT SaST]].
   generalize SGOOD; move=> [[SGMEM [SGREG SGPC]] SGINT].
-  generalize AGOOD =>
-    /andP [/andP [/andP [AELEM /andP [/andP [AGOODS ANOL] ACC]] ASS] ASP];
-    assert (AIN : In Aprev AC) by by simpl in *; destruct (elem Aprev AC).
+  case/and4P: (AGOOD) => AIN /andP [ANOL ACC] ASS ASP.
   rewrite /Abs.semantics /Abs.add_to_jump_targets
           /Abs.add_to_compartment_component
           (lock Abs.in_compartment_opt);
     simpl in *.
-
   rewrite /refine_pc_b in RPC.
   destruct Spc as [pc [F cid'| |]]; try done; move/eqP in RPC; subst.
 
@@ -1087,7 +1088,7 @@ Proof.
     undo1 ADD s';
     undo2 ADD pc' Lpc';
     undoDATA ADD i' cid_next I_next W_next;
-    undo1 ADD NEXT_EQ; move/eqP in NEXT_EQ; subst cid_next.
+    undo1 ADD NEXT_EQ; move/eqP in NEXT_EQ; subst cid_next;
     undo1 ADD NEXT;
     destruct s' as [M_next R_next not_pc si_next];
     unoption.
@@ -1096,17 +1097,17 @@ Proof.
     rewrite /refine_compartments /refine_compartment_tag /= in RCOMP;
     move: RCOMP => [RCOMPS RCTAGS] RCOMP.
   move: (RCTAGS pc) => RCTAGS'; rewrite def_i_LI in RCTAGS';
-    destruct RCTAGS' as [SET_I [SET_W [c_sys [IN_c RTAG]]]].
+    destruct RCTAGS' as [c_sys [IN_c RTAG]].
 
-  assert (PNI : Abs.permitted_now_in AC Ask Aprev pc ?= c_sys) by
-    (eapply prove_permitted_now_in; eassumption);
-    rewrite PNI; simpl.
-  assert (R_c_sys : refined_compartment
+  have -> /=: Abs.permitted_now_in AC Ask Aprev pc ?= c_sys.
+    eapply prove_permitted_now_in; eassumption.
+
+  have R_c_sys: refined_compartment
                       c_sys
                       (SState SM SR pc@(Sym.PC F cid')
                               (SInternal Snext SiT SaJT SaST))
-                    == Some cid_sys)
-    by (eapply prove_refined_compartment' with (pc := pc); try eassumption).
+                    == Some cid_sys.
+    by eapply prove_refined_compartment' with (pc := pc); eassumption.
 
   rewrite /Sym.good_pc_tag in SGPC; move: SGPC => [p' [x' [I' [W' def_cid']]]].
   move: RPREV => /andP [/eqP? RPREV]; subst.
@@ -1125,9 +1126,13 @@ Proof.
     move/eqP in RREGS'; subst; simpl.
 
   destruct Aprev as [Aprev Jprev Sprev]; simpl.
-  assert (IC_p' : AC ⊢ p' ∈ <<Aprev,Jprev,Sprev>>). {
+  have IC_p' : AC ⊢ p' ∈ <<Aprev,Jprev,Sprev>>. {
     (* This lemma's proof cribbed from a lemma in `prove_permitted_now_in'. *)
-    move/eqP in RPREV; explode_refined_compartment' RPREV.
+    move/eqP: RPREV.
+    rewrite /refined_compartment.
+    case: pickP => // sc /andP [/eqP ? /forallP ?] [E]. subst sc.
+    admit.
+    (*; explode_refined_compartment' RPREV.
     move/id in def_sxs; move/id in MAP_sxs;
       move/id in SAME_cid; move/id in NE_cids.
     destruct cids as [|temp_cid cids];
@@ -1148,10 +1153,11 @@ Proof.
     assert (IC_p''_prev : AC ⊢ p'' ∈ <<Aprev,Jprev,Sprev>>) by
       by apply Abs.in_compartment_spec.
     replace c''' with <<Aprev,Jprev,Sprev>> in * by eauto 3.
-    assumption.
+    assumption. *)
   }
-  assert (IN_p : In p Aprev \/ In p Jprev). {
+  have ->: p \in Aprev :|: Jprev. {
     (* This lemma's proof cribbed from `prove_permitted_now_in'. *)
+    admit. (*
     move/eqP in RPREV; explode_refined_compartment' RPREV.
     move/id in def_xcIW; move/id in OK.
     move: (RCTAGS p) => RCTAGS'; rewrite def_xcIW /= in RCTAGS';
@@ -1176,13 +1182,15 @@ Proof.
       specialize RTAG''' with p; rewrite def_xcIW in RTAG'''.
       move: RTAG''' => [_ [IN_I _]].
       apply set_elem_true, IN_I in IN_I''; auto.
-      by replace c''' with <<Aprev,Jprev,Sprev>> in * by eauto 3.
+      by replace c''' with <<Aprev,Jprev,Sprev>> in * by eauto 3.*)
   }
+  (*
   have -> : set_elem p (set_union Aprev Jprev). {
     assert (Abs.good_compartment <<Aprev,Jprev,Sprev>>) by eauto 2.
     apply set_elem_true;
       [apply set_union_preserves_set; eauto 2 | by apply set_union_spec].
   }
+  *)
 
   generalize RREGS => RREGS';
     rewrite /refine_registers /pointwise /refine_reg_b in RREGS';
@@ -1207,7 +1215,7 @@ Proof.
   }
   assert (IC_pc' : AC ⊢ pc' ∈ <<Aprev,Jprev,Sprev>>). {
     specialize RCTAGS with p'; rewrite def_cid' in RCTAGS.
-    move: RCTAGS => [_ [_ [c_temp [IC_temp RTAG']]]].
+    move: RCTAGS => [c_temp [IC_temp RTAG']].
     replace c_temp with <<Aprev,Jprev,Sprev>> in * by eauto 3; simpl in *.
     specialize RTAG' with pc'.
     remember (Sym.sget _ pc') as v eqn:SGET in RTAG'; symmetry in SGET.
@@ -1220,13 +1228,11 @@ Proof.
       inversion EQUICOMPARTMENTAL; subst; clear EQUICOMPARTMENTAL.
     by destruct RTAG' as [SAME _]; apply SAME.
   }
-  assert (IN_pc' : In pc' Aprev) by
-    (apply Abs.in_compartment_spec in IC_pc'; tauto).
-  assert (ELEM_pc' : set_elem pc' Aprev) by
-    (move/forallb_forall in AGOODS; apply set_elem_true; eauto 3).
-  rewrite -(lock Abs.in_compartment_opt) /= ELEM_pc' /= eq_refl.
+  assert (IN_pc' : pc' \in Aprev) by admit. (* trivial *)
+  rewrite -(lock Abs.in_compartment_opt) /= IN_pc' /= eq_refl.
 
-  assert (IN_Jsys : In pc' (Abs.jump_targets c_sys)). {
+  have IN_Jsys : pc' \in Abs.jump_targets c_sys. {
+    admit. (*
     undo1 def_cid_sys COND; unoption.
     apply set_elem_true in NEXT.
     - destruct (pc' == p) eqn:EQ; move/eqP in EQ; [subst p|].
@@ -1251,13 +1257,10 @@ Proof.
         move: SGMEM => /andP []; auto.
       + eapply Sym.sget_supd_neq in def_s'; eauto 1.
         rewrite -def_s' def_xcIW0 in SGMEM.
-        move: SGMEM => /andP [] //.
+        move: SGMEM => /andP [] //. *)
   }
-  have -> : set_elem pc' (Abs.jump_targets c_sys) by
-    (apply Abs.in_compartment_spec in IN_c; destruct IN_c;
-     move/forallb_forall in AGOODS; apply set_elem_true; eauto 3).
 
-  eexists; split; [reflexivity|].
+  rewrite IN_Jsys. eexists; split; [reflexivity|].
 
   assert (sget_next_spec : forall a,
             Sym.sget (SState M_next R_next not_pc si_next) a =
@@ -1266,7 +1269,7 @@ Proof.
 
             \/
             (Sym.sget (SState M_next R_next not_pc si_next) a ?=
-               x@(Sym.DATA cid'' (insert_unique cid' I'') W'') /\
+               x@(Sym.DATA cid'' (cid' |: I'') W'') /\
              p = a))
     by abstract
          (intros a; destruct (a == p) eqn:EQ; move/eqP in EQ; subst;
@@ -1275,7 +1278,7 @@ Proof.
 
   assert (M_next_spec : forall a,
             get M_next a = get SM a \/
-            (get M_next a ?= x@(Sym.DATA cid'' (insert_unique cid' I'') W'')  /\
+            (get M_next a ?= x@(Sym.DATA cid'' (cid' |: I'') W'')  /\
              p = a)).
   {
     intros a; destruct (a == p) eqn:EQ; move/eqP in EQ; subst.
@@ -1328,12 +1331,7 @@ Proof.
             have [->|/eqP NEQ] := altP (p'' =P p).
             - rewrite /Sym.good_memory_tag /Sym.sget /sst'.
               generalize (PartMaps.get_upd_eq UPD) => EQ.
-              rewrite EQ.
-              move: GOOD => /(_ p) GOOD.
-              rewrite /Sym.good_memory_tag /sst def_xcIW in GOOD.
-              move/andP: GOOD => [GOOD1 GOOD2].
-              apply/andP. split; last by [].
-              by apply insert_unique_preserves_set_true.
+              by rewrite EQ.
             - rewrite /Sym.good_memory_tag /Sym.sget /sst'.
               generalize (PartMaps.get_upd_neq NEQ UPD) => EQ.
               rewrite EQ.
@@ -1348,7 +1346,7 @@ Proof.
               rewrite /Sym.sget /sst' EQ.
               split; first by [].
               split; last by [].
-              move => a. apply insert_unique_preserves.
+              exact: subsetUr.
             - generalize (PartMaps.get_upd_neq NEQ UPD) => EQ.
               rewrite /Sym.sget /sst /sst' EQ.
               move: GOOD => /(_ p'') GOOD.
@@ -1360,24 +1358,19 @@ Proof.
               case: (p'' == add_to_store_targets_addr); by [case SaST | ]. }
           rewrite /tags_subsets in COMPAT.
           rename Aprev into A; rename Jprev into J; rename Sprev into S.
-
-          assert (INIT :
-            (do! sxs <- map_options (Sym.sget sst) A;
-             the =<< map_options (Sym.stag_compartment ∘ slabel) sxs)
-            =
-            (do! sxs' <- map_options (Sym.sget sst') A;
-             the =<< map_options (Sym.stag_compartment ∘ slabel) sxs')).
+          have INIT : (Sym.stag_compartment ∘ slabel <=< Sym.sget sst)  @: A =
+                      (Sym.stag_compartment ∘ slabel <=< Sym.sget sst') @: A.
           {
-            clear AELEM AIN AGOOD SYS_SEP IC_p' IN_p PNI IC_pc' IN_pc'
-                  ELEM_pc'.
-            rewrite (lock the) 2!bind_assoc -(lock the) 2!map_options_bind;
+            clear AIN AGOOD SYS_SEP IC_p' IC_pc' IN_pc'.
+            admit. (*
+            rewrite 2!bind_assoc -(lock the) 2!map_options_bind;
               f_equal.
             induction A as [|a A]; simpl in *; [reflexivity|].
             specialize COMPAT with a.
             destruct (Sym.sget sst  a) as [[z  [|cz  Iz  Wz|]]|],
                      (Sym.sget sst' a) as [[z' [|cz' Iz' Wz'|]]|];
               try done; destruct COMPAT as [EQ _]; subst; simpl.
-            rewrite IHA; try done.
+            rewrite IHA; try done. *)
           }
 
           intros REFINED; rewrite bind_assoc in REFINED.
